New atomic updates: defined as a fixed point with existential quantifier; intro lemma using class of Laterable assertions

theories/bi/lib/atomic.v
@@ -1,48 +1,109 @@
 From iris.bi Require Export bi updates.
+From iris.bi.lib Require Import fixpoint laterable.
 From stdpp Require Import coPset.
 From iris.proofmode Require Import tactics.
 Set Default Proof Using "Type".
 
-Definition atomic_shift `{BiFUpd PROP} {A B : Type}
-  (α : A → PROP) (* atomic pre-condition *)
-  (β : A → B → PROP) (* atomic post-condition *)
-  (Eo Em : coPset) (* outside/module masks *)
-  (P : PROP) (* pre-condition *)
-  (Q : A → B → PROP) (* post-condition *)
-  : PROP :=
-    (□ (∀ E, ⌜Eo ⊆ E⌝ -∗ P ={E, E∖Em}=∗ ∃ x, α x ∗
-          ((α x ={E∖Em, E}=∗ P) ∧ (∀ y, β x y ={E∖Em, E}=∗ Q x y)))
+(** atomic_update as a fixed-point of the equation
+   AU = ∃ P. ▷ P ∗ □ (▷ P ==∗ α ∗ (α ==∗ AU) ∧ (β ==∗ Q))
+ *)
+Section definition.
+  Context `{BiFUpd PROP} {A B : Type}
+    (α : A → PROP) (* atomic pre-condition *)
+    (β : A → B → PROP) (* atomic post-condition *)
+    (Eo Em : coPset) (* outside/module masks *)
+    (Φ : A → B → PROP) (* post-condition *)
+  .
+
+  Definition atomic_shift (P P' : PROP) : PROP :=
+    (□ (∀ E, ⌜Eo ⊆ E⌝ → P ={E, E∖Em}=∗ ∃ x, α x ∗
+          ((α x ={E∖Em, E}=∗ P') ∧ (∀ y, β x y ={E∖Em, E}=∗ Φ x y)))
     )%I.
 
-Definition atomic_update `{BiFUpd PROP} {A B : Type}
-  (α : A → PROP) (* atomic pre-condition *)
-  (β : A → B → PROP) (* atomic post-condition *)
-  (Eo Em : coPset) (* outside/module masks *)
-  (Q : A → B → PROP) (* post-condition *)
-  : PROP :=
-    tc_opaque (
-      ∃ (F P : PROP), F ∗ ▷ P ∗ atomic_shift α β Eo Em (▷ P) (λ x y, F -∗ Q x y)
-    )%I.
-
-Section lemmas.
-  Context `{BiFUpd PROP} {A B : Type}.
-  Implicit Types (α : A → PROP) (β: A → B → PROP) (P : PROP) (Q : A → B → PROP).
-
-  Lemma aupd_acc α β Eo Em Q E :
-    Eo ⊆ E →
-    atomic_update α β Eo Em Q -∗
-    |={E, E∖Em}=> ∃ x, α x ∗
-      ((α x ={E∖Em, E}=∗ atomic_update α β Eo Em Q) ∧
-       (∀ y, β x y ={E∖Em, E}=∗ Q x y)).
-  Proof using Type*.
-    rewrite {1}/atomic_update /=. iIntros (HE) "HUpd".
-    iDestruct "HUpd" as (F P) "(HF & HP & #Hshift)".
-    iMod ("Hshift" with "[% //] HP") as (x) "[Hα Hclose]".
+  Lemma atomic_shift_mono P P1 P2:
+    □ (P1 -∗ P2) -∗ □ (atomic_shift P P1 -∗ atomic_shift P P2).
+  Proof.
+    iIntros "#HP12 !# #AS !# * % HP".
+    iMod ("AS" with "[% //] HP") as (x) "[Hα Hclose]".
     iModIntro. iExists x. iFrame "Hα". iSplit.
     - iIntros "Hα". iDestruct "Hclose" as "[Hclose _]".
-      iMod ("Hclose" with "Hα"). iModIntro. iExists F, P.
-      by iFrame.
+      iApply "HP12". iApply "Hclose". done.
     - iIntros (y) "Hβ". iDestruct "Hclose" as "[_ Hclose]".
-      iMod ("Hclose" with "Hβ") as "HQ". iModIntro. by iApply "HQ".
+      iApply "Hclose". done.
+  Qed.
+
+  Definition atomic_update_pre (Ψ : () → PROP) (_ : ()) : PROP :=
+    (∃ (P : PROP), ▷ P ∗ atomic_shift (▷ P) (Ψ ()))%I.
+
+  Local Instance atomic_update_pre_mono : BiMonoPred atomic_update_pre.
+  Proof.
+    constructor.
+    - iIntros (P1 P2) "#HP12". iIntros ([]) "AU".
+      iDestruct "AU" as (P) "[HP AS]". iExists P. iFrame.
+      iApply (atomic_shift_mono with "[HP12]"); last done.
+      iAlways. iApply "HP12".
+    - intros ??. solve_proper.
+  Qed.
+
+  Definition atomic_update_def :=
+    bi_greatest_fixpoint atomic_update_pre ().
+End definition.
+
+(** Seal it *)
+Definition atomic_update_aux : seal (@atomic_update_def). by eexists. Qed.
+Definition atomic_update `{BiFUpd PROP} {A B : Type} := atomic_update_aux.(unseal) PROP _ A B.
+Definition atomic_update_eq :
+  @atomic_update = @atomic_update_def := atomic_update_aux.(seal_eq).
+
+(** Lemmas about AU *)
+Section lemmas.
+  Context `{BiFUpd PROP} {A B : Type}.
+  Implicit Types (α : A → PROP) (β: A → B → PROP) (P : PROP) (Φ : A → B → PROP).
+
+  Local Existing Instance atomic_update_pre_mono.
+
+  (** The ellimination form: an accessor *)
+  Lemma aupd_acc α β Eo Em Φ E :
+    Eo ⊆ E →
+    atomic_update α β Eo Em Φ -∗
+    |={E, E∖Em}=> ∃ x, α x ∗
+      ((α x ={E∖Em, E}=∗ atomic_update α β Eo Em Φ) ∧
+       (∀ y, β x y ={E∖Em, E}=∗ Φ x y)).
+  Proof using Type*.
+    rewrite atomic_update_eq {1}/atomic_update_def /=. iIntros (HE) "HUpd".
+    iPoseProof (greatest_fixpoint_unfold_1 with "HUpd") as "HUpd".
+    iDestruct "HUpd" as (P) "(HP & Hshift)".
+    iMod ("Hshift" with "[% //] HP") as (x) "[Hα Hclose]".
+    iModIntro. iExists x. iFrame.
+  Qed.
+
+  Global Instance aupd_laterable α β Eo Em Φ :
+    Laterable (atomic_update α β Eo Em Φ).
+  Proof.
+    rewrite /Laterable atomic_update_eq {1}/atomic_update_def /=. iIntros "AU".
+    iPoseProof (greatest_fixpoint_unfold_1 with "AU") as (P) "[HP #AS]".
+    iExists P. iFrame. iIntros "!# HP !>".
+    iApply greatest_fixpoint_unfold_2. iExists P. iFrame "#∗".
+  Qed.
+
+  Lemma aupd_intro P α β Eo Em Φ :
+    Em ⊆ Eo → Laterable P →
+    P -∗
+    □ (P -∗ |={Eo, Eo∖Em}=> ∃ x, α x ∗
+      ((α x ={Eo∖Em, Eo}=∗ P) ∧ (∀ y, β x y ={Eo∖Em, Eo}=∗ Φ x y))) -∗
+    atomic_update α β Eo Em Φ.
+  Proof.
+    rewrite atomic_update_eq {1}/atomic_update_def /=.
+    iIntros (??) "HP #AU".
+    iApply (greatest_fixpoint_coind _ (λ _, P)); last done. iIntros "!#" ([]) "HP".
+    iDestruct (laterable with "HP") as (P') "[HP' #HPi]". iExists P'. iFrame.
+    iIntros "!#" (E HE) "HP'". iDestruct ("HPi" with "HP'") as ">HP {HPi}".
+    iApply fupd_mask_frame_diff_open; last
+      iMod ("AU" with "HP") as (x) "[Hα Hclose] {AU}"; [done..|].
+    iModIntro. iExists x. iFrame. iSplit.
+    - iDestruct "Hclose" as "[Hclose _]". iIntros "Hα".
+      iApply fupd_mask_frame_diff_close; last (by iApply "Hclose"); done.
+    - iDestruct "Hclose" as "[_ Hclose]". iIntros (y) "Hβ".
+      iApply fupd_mask_frame_diff_close; last (by iApply "Hclose"); done.
   Qed.
 End lemmas.
