theories/bi/lib/laterable.v
@@ -1,0 +1,53 @@
+From iris.bi Require Export bi.
+From iris.proofmode Require Import tactics.
+Set Default Proof Using "Type".
+
+(** The class of laterable assertions *)
+Class Laterable {PROP : sbi} (P : PROP) := laterable :
+  P -∗ ∃ Q, ▷ Q ∗ □ (▷ Q -∗ ◇ P).
+Arguments Laterable {_} _%I : simpl never.
+Arguments laterable {_} _%I {_}.
+Hint Mode Laterable + ! : typeclass_instances.
+
+Section instances.
+  Context {PROP : sbi}.
+  Implicit Type (P : PROP).
+
+  Global Instance later_laterable P : Laterable (▷ P).
+  Proof.
+    rewrite /Laterable. iIntros "HP". iExists P. iFrame.
+    iIntros "!# HP !>". done.
+  Qed.
+
+  Global Instance timeless_laterable P :
+    Timeless P → Laterable P.
+  Proof.
+    rewrite /Laterable. iIntros (?) "HP". iExists P%I. iFrame.
+    iSplitR; first by iNext. iIntros "!# >HP !>". done.
+  Qed.
+
+  (** This lemma is not very useful: It needs a strange assumption about
+      emp, and most of the time intuitionistic propositions can be just kept
+      around anyway and don't need to be "latered".  The lemma exists
+      because the fact that it needs the side-condition is interesting;
+      it is not an instance because it won't usually get used. *)
+  Lemma intuitionistic_laterable P :
+    Timeless (PROP:=PROP) emp → Affine P → Persistent P → Laterable P.
+  Proof.
+    rewrite /Laterable. iIntros (???) "#HP".
+    iExists emp%I. iSplitL; first by iNext.
+    iIntros "!# >_". done.
+  Qed.
+
+  Global Instance sep_laterable P Q :
+    Laterable P → Laterable Q → Laterable (P ∗ Q).
+  Proof.
+    rewrite /Laterable. iIntros (LP LQ) "[HP HQ]".
+    iDestruct (LP with "HP") as (P') "[HP' #HP]".
+    iDestruct (LQ with "HQ") as (Q') "[HQ' #HQ]".
+    iExists (P' ∗ Q')%I. iSplitL; first by iFrame.
+    iIntros "!# [HP' HQ']". iSplitL "HP'".
+    - iApply "HP". done.
+    - iApply "HQ". done.
+  Qed.
+End instances.
